floyd/loadstore_field_at.v
@@ -9,7 +9,6 @@ Require Import VST.floyd.reptype_lemmas.
 Require Import VST.floyd.data_at_rec_lemmas.
 Require Import VST.floyd.field_at.
 Require Import VST.floyd.loadstore_mapsto.
-
 Import LiftNotation.
 
 Lemma is_neutral_cast_by_value: forall t t',
